progress on COSE

share/pulse/examples/dice/cbor/COSE.AST.fst
@@ -4,21 +4,37 @@ module Spec = COSE.Spec
 
 #set-options "--fuel 0"
 
+[@@ bounded_attr; sem_attr]
 let e0 = empty_env
 let thr0 : spec_array_group_splittable_threshold e0 = spec_array_group_splittable_threshold_empty _
 
-let e1 = env_extend_map_group e0 "header_map0" Spec.header_map0 ()
-
-let e2 = env_extend_typ e1 "header_map" (TElem (TMap "header_map0")) ()
-
-let e3 = env_extend_typ e2 "empty_or_serialized_map" (TEscapeHatch Spec.empty_or_serialized_map) ()
-
-let e4 =
-  env_extend_array_group e3 "headers" [
-    "protected", TAAtom (TAElem (TDef "empty_or_serialized_map"));
-    "unprotected", TAAtom (TAElem (TDef "header_map"));
-  ]
+[@@ bounded_attr; sem_attr]
+let e1 = env_extend_map_group e0 "header_map0" 
   (_ by (solve_env_extend_array_group ()))
+  Spec.header_map0
+  (_ by (solve_env_extend_array_group ()))
+
+[@@ bounded_attr; sem_attr]
+let e2 = env_extend_typ e1 "header_map"
+  (_ by (solve_env_extend_array_group ()))
+  (TElem (TMap "header_map0"))
+  (_ by (solve_env_extend_array_group ()))
+
+[@@ bounded_attr; sem_attr]
+let e3 = env_extend_typ e2 "empty_or_serialized_map"
+  (_ by (solve_env_extend_array_group ()))
+  (TEscapeHatch Spec.empty_or_serialized_map)
+  (_ by (solve_env_extend_array_group ()))
+
+[@@ bounded_attr; sem_attr]
+let e4 =
+  env_extend_array_group e3 "headers"
+    (_ by (solve_env_extend_array_group ()))
+    [
+      "protected", TAAtom (TAElem (TDef "empty_or_serialized_map"));
+      "unprotected", TAAtom (TAElem (TDef "header_map"));
+    ]
+    (_ by (solve_env_extend_array_group ()))
 
 let thr4 : spec_array_group_splittable_threshold e4 =
   spec_array_group_splittable_threshold_extend
@@ -33,18 +49,104 @@ let _ : squash (
   assert (array_group_sem e4.e_semenv a `CDDL.Spec.array_group3_equiv` Spec.headers)
     by (solve_sem_equiv ())
 
+[@@ bounded_attr; sem_attr]
 let e5 =
-  env_extend_typ e4 "bstr" (TEscapeHatch CDDL.Spec.bstr) ()
+  env_extend_typ e4 "bstr"
+    (_ by (solve_env_extend_array_group ()))
+    (TEscapeHatch CDDL.Spec.bstr)
+    (_ by (solve_env_extend_array_group ()))
 
+[@@ bounded_attr; sem_attr]
 let e6 =
-  env_extend_array_group e5 "cose_signature0" [
-    "headers", TAAtom (TADef "headers");
-    "signature", TAAtom (TAElem (TDef "bstr"));
-  ]
-  (_ by (solve_env_extend_array_group ()))
+  env_extend_array_group e5 "cose_signature_array"
+    (_ by (solve_env_extend_array_group ()))
+    [
+      "headers", TAAtom (TADef "headers");
+      "signature", TAAtom (TAElem (TDef "bstr"));
+    ]
+    (_ by (solve_env_extend_array_group ()))
 
 let thr6 : spec_array_group_splittable_threshold e6 =
   spec_array_group_splittable_threshold_extend
     (spec_array_group_splittable_threshold_extend_env thr4 e6)
-    "cose_signature0"
+    "cose_signature_array"
     (_ by (solve_spec_array_group_splittable ()))
+
+[@@ bounded_attr; sem_attr]
+let e7 =
+  env_extend_typ e6 "cose_signature"
+    (_ by (solve_env_extend_array_group ()))
+    (TElem (TArray "cose_signature_array"))
+    (_ by (solve_env_extend_array_group ()))
+
+let _ : squash (
+  se_typ e7.e_semenv "cose_signature" `CDDL.Spec.typ_equiv` Spec.cose_signature
+) = 
+  let a = normalize_term (e7.e_env "cose_signature") in
+  assert (typ_sem e7.e_semenv a `CDDL.Spec.typ_equiv` Spec.cose_signature)
+    by (solve_sem_equiv ())
+
+[@@ bounded_attr; sem_attr]
+let e8 =
+  env_extend_typ e7 "cose_signature_payload" 
+    (_ by (solve_env_extend_array_group ()))
+    (TChoice [
+      TByteString;
+      TNil;
+    ])
+    (_ by (solve_env_extend_array_group ()))
+
+[@@ bounded_attr; sem_attr]
+let e9 =
+  env_extend_array_group e8 "cose_signatures"
+    (_ by (solve_env_extend_array_group ()))
+    ["signatures", TAOneOrMore (TAElem (TDef "cose_signature"))]
+    (_ by (solve_env_extend_array_group ()))
+
+let thr9 : spec_array_group_splittable_threshold e9 =
+  spec_array_group_splittable_threshold_extend
+    (spec_array_group_splittable_threshold_extend_env thr6 e9)
+    "cose_signatures"
+    (_ by (solve_spec_array_group_splittable ()))
+
+[@@ bounded_attr; sem_attr]
+let e10 =
+  env_extend_array_group e9 "cose_sign_array"
+    (_ by (solve_env_extend_array_group ()))
+    [
+      "headers", TAAtom (TADef "headers");
+      "payload", TAAtom (TAElem (TDef "cose_signature_payload"));
+      "signatures", TAAtom (TAElem (TArray "cose_signatures"));
+    ]
+    (_ by (solve_env_extend_array_group ()))
+
+let thr10 : spec_array_group_splittable_threshold e10 =
+  spec_array_group_splittable_threshold_extend
+    (spec_array_group_splittable_threshold_extend_env thr9 e10)
+    "cose_sign_array"
+    (_ by (solve_spec_array_group_splittable ()))
+
+#push-options "--z3rlimit 16" // cannot reason about GSet
+
+[@@ bounded_attr; sem_attr]
+let e11 =
+  env_extend_typ e10 "cose_sign"
+    (_ by (solve_env_extend_array_group ()))
+    (TElem (TArray "cose_sign_array"))
+    (_ by (solve_env_extend_array_group ()))
+
+#push-options "--z3rlimit 32" // cannot reason about typ_equiv
+
+let _ : squash (
+  se_typ e11.e_semenv "cose_sign" `CDDL.Spec.typ_equiv` Spec.cose_sign
+) = 
+  let a = normalize_term (e11.e_env "cose_sign") in
+  assert (typ_sem e11.e_semenv a `CDDL.Spec.typ_equiv` Spec.cose_sign)
+    by (solve_sem_equiv ())
+
+[@@ bounded_attr; sem_attr]
+let e12 =
+  env_extend_typ e11 "cose_sign_tagged"
+    (_ by (solve_env_extend_array_group ()))
+    (TTag Spec.tag_cose_sign (TDef "cose_sign"))
+    (_ by (solve_env_extend_array_group ()))
